consolidate list examples

Examples/llistR.v
@@ -10,19 +10,16 @@ Obligation Tactic := auto.
 
 (* linked lists, storing a value and next pointer in consecutive locations *)
 
-Definition llist (T : Type) := ptr.
-
-Section LList.
-Variable T : Type.
-Notation llist := (llist T).
-
-Fixpoint lseg (p q : ptr) (xs : seq T) :=
+Fixpoint lseg {A} (p q : ptr) (xs : seq A) :=
   if xs is hd::tl then
     [Pred h | exists r h',
        h = (p :-> hd) \+ (p .+ 1 :-> r \+ h') /\ h' \In lseg r q tl]
   else [Pred h | p = q /\ h = Unit].
 
-Lemma lseg_add_last xs x p r h :
+Section LSeg.
+Variable A : Type.
+
+Lemma lseg_add_last (xs : seq A) x p r h :
         h \In lseg p r (rcons xs x) <->
         exists q h', h = h' \+ (q :-> x \+ q .+ 1 :-> r) /\ h' \In lseg p q xs.
 Proof.
@@ -36,7 +33,7 @@ exists z, (h2 \+ q :-> y \+ q .+ 1 :-> r).
 by rewrite -!joinA; split=>//; apply/IH; eauto.
 Qed.
 
-Lemma lseg_null xs q h :
+Lemma lseg_null (xs : seq A) q h :
          valid h -> h \In lseg null q xs ->
          [/\ q = null, xs = [::] & h = Unit].
 Proof.
@@ -44,7 +41,7 @@ case: xs=>[|x xs] D /= H; first by case: H=><- ->.
 case: H D=>r [h'][->] _; rewrite validPtUn; hhauto.
 Qed.
 
-Lemma lseg_neq xs p q h :
+Lemma lseg_neq (xs : seq A) p q h :
         p != q -> h \In lseg p q xs ->
         exists x r h',
          [/\ xs = x :: behead xs, p :-> x \+ (p .+ 1 :-> r \+ h') = h &
@@ -54,12 +51,12 @@ case: xs=>[|x xs] /= H []; last by move=>y [h'][->] H1; hhauto.
 by move=>E; rewrite E eq_refl in H.
 Qed.
 
-Lemma lseg_empty xs p q : Unit \In lseg p q xs -> p = q /\ xs = [::].
+Lemma lseg_empty (xs : seq A) p q : Unit \In lseg p q xs -> p = q /\ xs = [::].
 Proof.
 by case: xs=>[|x xs][] // r [h][/esym/join0E][/unitbE]; rewrite /heap_pts ptsU um_unitbU.
 Qed.
 
-Lemma lseg_case xs p q h :
+Lemma lseg_case (xs : seq A) p q h :
         h \In lseg p q xs ->
         [/\ p = q, xs = [::] & h = Unit] \/
         exists x r h',
@@ -70,20 +67,25 @@ case: xs=>[|x xs] /=; first by case=>->->; left.
 by case=>r [h'][->] H; right; hhauto.
 Qed.
 
-(* Special case when p = null *)
-Definition lseq p := lseg p null.
+End LSeg.
 
-Lemma lseq_null xs h : valid h -> h \In lseq null xs -> xs = [::] /\ h = Unit.
+(* Special case when p = null *)
+Definition lseq {A} p (xs : seq A) := lseg p null xs.
+
+Section LList.
+Variable A : Type.
+
+Lemma lseq_null (xs : seq A) h : valid h -> h \In lseq null xs -> xs = [::] /\ h = Unit.
 Proof. by move=>D; case/(lseg_null D)=>_ ->. Qed.
 
-Lemma lseq_pos xs p h :
+Lemma lseq_pos (xs : seq A) p h :
         p != null -> h \In lseq p xs ->
         exists x r h',
           [/\ xs = x :: behead xs,
               p :-> x \+ (p .+ 1 :-> r \+ h') = h & h' \In lseq r (behead xs)].
 Proof. by apply: lseg_neq. Qed.
 
-Lemma lseq_func l1 l2 p h : valid h -> h \In lseq p l1 -> h \In lseq p l2 -> l1 = l2.
+Lemma lseq_func (l1 l2 : seq A) p h : valid h -> h \In lseq p l1 -> h \In lseq p l2 -> l1 = l2.
 Proof.
 elim: l1 l2 p h => [|x1 xt IH] /= l2 p h V.
 - by case=>->->; case/lseq_null.
@@ -96,7 +98,7 @@ Qed.
 (* main methods *)
 
 (* prepending *)
-Program Definition insert p x :
+Program Definition insert p (x : A) :
   {l}, STsep (lseq p l, [vfun p' => lseq p' (x::l)]) :=
   Do (q <-- allocb p 2;
       q ::= x;;
@@ -109,7 +111,7 @@ Qed.
 
 (* removing *)
 
-Program Definition remove p : {xs}, STsep (lseq p xs, [vfun p' => lseq p' (behead xs)]) :=
+Program Definition remove p : {xs : seq A}, STsep (lseq p xs, [vfun p' => lseq p' (behead xs)]) :=
   Do (if p == null then ret p
       else pnext <-- !(p .+ 1);
            dealloc p;;
@@ -126,9 +128,9 @@ Qed.
 (* length *)
 
 Definition lenT : Type :=
-  forall (pl : ptr * nat), {xs}, STsep (lseq pl.1 xs, [vfun l h => l == pl.2 + length xs /\ lseq pl.1 xs h]).
+  forall (pl : ptr * nat), {xs : seq A}, STsep (lseq pl.1 xs, [vfun l h => l == pl.2 + length xs /\ lseq pl.1 xs h]).
 
-Program Definition len p : {xs}, STsep (lseq p xs, [vfun l h => l == length xs /\ lseq p xs h]) :=
+Program Definition len p : {xs : seq A}, STsep (lseq p xs, [vfun l h => l == length xs /\ lseq p xs h]) :=
   Do (let: len := Fix (fun (go : lenT) '(p, l) =>
                         Do (if p == null then ret l
                             else pnext <-- !(p .+ 1);
@@ -154,11 +156,11 @@ Qed.
 (* concatenation *)
 
 Definition catT (p2 : ptr) : Type :=
-  forall (p1 : ptr), {xs}, STsep (fun h => p1 != null /\ (lseq p1 xs.1 # lseq p2 xs.2) h,
-                                 [vfun _ : unit => lseq p1 (xs.1 ++ xs.2)]).
+  forall (p1 : ptr), {xs : seq A * seq A}, STsep (fun h => p1 != null /\ (lseq p1 xs.1 # lseq p2 xs.2) h,
+                                                 [vfun _ : unit => lseq p1 (xs.1 ++ xs.2)]).
 
-Program Definition concat p1 p2 : {xs1 xs2}, STsep (lseq p1 xs1 # lseq p2 xs2,
-                                                    [vfun a => lseq a (xs1 ++ xs2)]) :=
+Program Definition concat p1 p2 : {xs1 xs2 : seq A}, STsep (lseq p1 xs1 # lseq p2 xs2,
+                                                           [vfun a => lseq a (xs1 ++ xs2)]) :=
   Do (let: cat := Fix (fun (go : catT p2) q =>
                         Do (next <-- !(q .+ 1);
                             if (next : ptr) == null
@@ -199,12 +201,12 @@ Qed.
 
 (* in-place reversal *)
 
-Definition shape_rev p s := [Pred h | h \In lseq p.1 s.1 # lseq p.2 s.2].
+Definition shape_rev p (s : seq A * seq A) := [Pred h | h \In lseq p.1 s.1 # lseq p.2 s.2].
 
 Definition revT : Type := (* ps.1 = i, ps.2 = done *)
   forall p, {ps}, STsep (shape_rev p ps, [vfun y => lseq y (rev ps.1 ++ ps.2)]).
 
-Program Definition reverse p : {xs}, STsep (lseq p xs, [vfun p' => lseq p' (rev xs)]) :=
+Program Definition reverse p : {xs : seq A}, STsep (lseq p xs, [vfun p' => lseq p' (rev xs)]) :=
   Do (let: reverse := Fix (fun (go : revT) '(i, done) =>
                         Do (if i == null then ret done
                             else next <-- !i .+ 1;
@@ -223,6 +225,43 @@ Next Obligation.
 move=>p /=.
 apply: ghR=>i xs H _; apply: (gh_ex (xs, [::])).
 by apply: val_do0=>//; [exists i; hhauto | move=>x m /=; rewrite cats0].
+Qed.
+
+Variable B : Type.
+
+(* Type of recursive map *)
+Definition lmap_type (f : A -> B) :=
+  forall (p : ptr),
+    {xs : seq A}, STsep (lseq p xs,
+                         fun (_ : ans unit) => lseq p (map f xs)).
+
+Program Definition lmap f : lmap_type f :=
+  Fix (fun (lmap : lmap_type f) p =>
+    Do (if p == null
+        then ret tt
+        else t <-- !p;
+             p ::= f t;;
+             nxt <-- !p .+ 1;
+             lmap nxt)).
+Next Obligation.
+(* Deconstruct the precondition *)
+move=>f lmap p.
+apply: ghR=>h xs P V.
+
+(* Use if-rule *)
+case: ifP=>[X|/negbT X].
+
+(* 1. p == null ==> The list is empty. *)
+- move/eqP: X=>Z; rewrite {}Z in P *.
+  by case: (lseq_null V P)=>->->; heval.
+
+(* 2. p != null => The list is non-empty. *)
+case/(lseq_pos X): P=>t [nxt][h'][->]Z/=P; rewrite -{}Z in V *.
+(* Decompose the list predicate *)
+rewrite joinA joinC in V *; heval.
+apply: (gh_ex (behead xs)).
+by apply: (@val_do _ _ _ h')=>//=_ h2 Q V'; rewrite joinC;
+   exists nxt, h2; rewrite joinA.
 Qed.
 
 End LList.
